Prove initialization and uninterruptible waiting in a rendezvous

formal-proofs/theories/lib/asym_rendezvous/asym_rendezvous_proof.v
@@ -59,26 +59,19 @@ Proof. apply _. Qed.
 Theorem pass_permit_exclusive γ: pass_permit γ -∗ pass_permit γ -∗ False.
 Proof.
   iIntros "H1 H2". rewrite /pass_permit.
-  iDestruct (own_valid_2 with "H1 H2") as %HVal.
-  inversion HVal as [HVal' _]; simpl in *.
-  inversion HVal' as [_ HVal'']; simpl in *.
-  inversion HVal''.
+  iDestruct (own_valid_2 with "H1 H2") as %[[_ []] _].
 Qed.
 
 Theorem fetch_permit_exclusve γ: fetch_permit γ -∗ fetch_permit γ -∗ False.
 Proof.
   iIntros "H1 H2". rewrite /pass_permit.
-  iDestruct (own_valid_2 with "H1 H2") as %HVal.
-  inversion HVal as [HVal' _]; simpl in *.
-  inversion HVal' as [HVal'' _]; simpl in *.
-  inversion HVal''.
+  iDestruct (own_valid_2 with "H1 H2") as %[[[] _] _].
 Qed.
 
 Theorem cancelled_not_passed γ: passed γ -∗ cancelled γ -∗ False.
 Proof.
   iIntros "H1 H2". rewrite /pass_permit.
-  iDestruct (own_valid_2 with "H1 H2") as %HVal.
-  inversion HVal as [_ HVal']; simpl in *.
+  iDestruct (own_valid_2 with "H1 H2") as %[_ HVal'].
   assert (true = false). { apply HVal'; repeat econstructor. }
   discriminate.
 Qed.
@@ -87,11 +80,138 @@ Definition asym_rendezvous_inv P ℓ γ :=
    (* Neither reader no writer came yet. *)
   ((own γ (● ((Excl' (), Excl' ()), None)) ∗ ℓ ↦ NONEV) ∨
    (* The writer came and left the resource, but the reader didn't come. *)
-   (own γ (● ((Excl' (), None), Some (to_agree false))) ∗ (∃ v, ℓ ↦ RESUMEDV v ∗
-                                                                  P v)) ∨
+   (own γ (● ((Excl' (), None), Some (to_agree false))) ∗
+        (∃ v, ℓ ↦ RESUMEDV v ∗ P v)) ∨
    (* The reader came and broke the cannel; writer wasn't here. *)
    (own γ (● ((None, Excl' ()), Some (to_agree true))) ∗ ℓ ↦ CANCELLEDV) ∨
    (* Both have come; nothing interesting can happen now. *)
-   (∃ f, own γ (● ((None, None), Some f))))%I.
+   (∃ (f: bool), own γ (● ((None, None), Some (to_agree f)))))%I.
+
+Definition is_asym_rendezvous γ v P :=
+  (∃ (ℓ: loc), ⌜v = #ℓ⌝ ∧ inv N (asym_rendezvous_inv P ℓ γ))%I.
+
+Theorem init_exchange_spec ℓ P:
+    {{{ ∃ v, ℓ ↦ v }}}
+      init_exchange #ℓ
+    {{{ γ, RET #(); is_asym_rendezvous γ #ℓ P ∗
+                                        fetch_permit γ ∗ pass_permit γ }}}.
+Proof.
+  iIntros (Φ) "Hℓ HPost".
+  wp_lam.
+  iDestruct "Hℓ" as (v) "Hℓ".
+  rewrite -wp_fupd.
+  wp_store.
+  iMod (own_alloc (● ((Excl' (), Excl' ()), None) ⋅
+                     ◯ (Excl' (), None, None) ⋅
+                     ◯ (None, Excl' (), None))) as (γ) "HOwn".
+  1: {
+    apply auth_valid_discrete; simpl.
+    repeat (split; try done).
+    eexists; split.
+    done.
+    split; try done.
+  }
+  repeat rewrite own_op.
+  iDestruct "HOwn" as "[[HOwn Hfetch] Hpass]".
+  iMod (inv_alloc N _ (asym_rendezvous_inv P ℓ γ) with "[Hℓ HOwn]") as "HInv".
+  {
+    iNext. rewrite /asym_rendezvous_inv.
+    eauto with iFrame.
+  }
+  iModIntro. iApply "HPost".
+  rewrite /is_asym_rendezvous. iFrame. iExists _. iSplit; done.
+Qed.
+
+Theorem await_spec γ r P:
+    {{{ is_asym_rendezvous γ r P ∗ fetch_permit γ }}}
+      await r
+    {{{ sm, RET sm; P sm ∗ passed γ }}}.
+Proof.
+  iIntros (Φ) "[#HIsR Hfp] HPost".
+  iDestruct "HIsR" as (ℓ) "[% #HInv]". subst.
+  iLöb as "IH". wp_lam. wp_bind (!_)%E.
+  iInv N as "HInvO" "HInvC".
+  iDestruct "HInvO" as "[[>HOwn Hℓ]|[[>HOwn Hℓ]|[[>HOwn Hℓ]|H]]]".
+  - wp_load.
+    iMod ("HInvC" with "[HOwn Hℓ]") as "_"; first by iLeft; iFrame.
+    iModIntro.
+    wp_pures.
+    by iApply ("IH" with "Hfp").
+  - iDestruct "Hℓ" as (v) "[Hℓ HP]".
+    wp_load.
+    iMod (own_update_2 with "HOwn Hfp") as "[HOwn Hpassed]".
+    {
+      apply transitivity with (y:=(● (None, None, Some (to_agree false)))).
+      - apply auth_update_dealloc.
+        apply local_update_unital_discrete.
+        intros z HValid HEq.
+        split; auto.
+        destruct z as [[z1 z2] z3]; simpl in *.
+        inversion HEq as [[HEq1 HEq2] HEq3]; simpl in *.
+        destruct z1.
+        {
+          inversion HEq1 as [x y HContra|]. subst.
+          inversion HContra.
+        }
+        done.
+      - apply auth_update_core_id with (b := (None, None, Some (to_agree false))).
+        apply pair_core_id; apply _.
+        done.
+    }
+    iMod ("HInvC" with "[HOwn Hℓ]") as "_".
+    {
+      repeat iRight.
+      eauto.
+    }
+    iModIntro.
+    wp_pures.
+    iApply "HPost".
+    iFrame.
+  - rewrite /fetch_permit.
+    iDestruct (own_valid_2 with "HOwn Hfp") as %HH.
+    apply auth_valid_discrete in HH; simpl in HH.
+    exfalso.
+    inversion HH as [_ [a [HAgr [HLe HVal]]]].
+    apply to_agree_inj in HAgr.
+    destruct a as [[u u'] u0].
+    inversion HAgr as [[HAgr' _] _].
+    inversion HAgr'; simpl in *; subst.
+    inversion HLe as [x [[HContra _] _]].
+    destruct x as [[xu xu'] xu0].
+    simpl in *.
+    destruct xu; by inversion HContra.
+  - iDestruct "H" as (f) ">HOwn".
+    rewrite /fetch_permit.
+    iDestruct (own_valid_2 with "HOwn Hfp") as %HH.
+    apply auth_valid_discrete in HH; simpl in HH.
+    exfalso.
+    inversion HH as [_ [a [HAgr [HLe HVal]]]].
+    apply to_agree_inj in HAgr.
+    destruct a as [[u u'] u0].
+    inversion HAgr as [[HAgr' _] _].
+    inversion HAgr'; simpl in *; subst.
+    inversion HLe as [x [[HContra _] _]].
+    destruct x as [[xu xu'] xu0].
+    simpl in *.
+    destruct xu; by inversion HContra.
+Qed.
+
+(*
+  await_interruptibly_spec Ni γi handle N γ r P:
+    {{{ is_interrupt_handle Ni γi handle ∗
+                            is_asym_rendezvous N γ r P ∗
+                            fetch_permit γ }}}
+      await_interruptibly handle r
+    {{{ sm, RET sm; (∃ v, ⌜sm = (#false, RESUMEDV v)%V⌝ ∧ P v ∗ passed γ) ∨
+                    (∃ v, ⌜sm = (#true, RESUMEDV v)%V⌝ ∧ P v ∗ passed γ ∗
+                                                           interrupted γi) ∨
+                    (⌜sm = (#true, NONEV)%V⌝ ∧ cancelled γ)
+    }}};
+  pass_spec N γ r P v:
+    {{{ is_asym_rendezvous N γ r P ∗ pass_permit γ ∗ P v }}}
+      pass r v
+    {{{ sm, RET sm; ⌜sm = NONEV⌝ ∧ passed γ ∨
+                                    ⌜sm = CANCELLEDV⌝ ∧ P v ∗ cancelled γ}}}
+*)
 
 End asym_rendezvous_proof.
